theories/L/Functions/EnumInt.v
@@ -1,5 +1,5 @@
 From Undecidability.L.Tactics Require Import LTactics.
-Require Import PslBase.Base List.
+Require Import PslBase.Base List Datatypes.
 From Undecidability.L.Computability Require Import Enum.
 From Undecidability.L.Functions Require Import Encoding Equality.
 From Undecidability.L.Datatypes Require Import LNat Lists LProd.
