theories/L/Functions/Proc.v
@@ -1,4 +1,5 @@
 From Undecidability.L Require Export Computability.Decidability Datatypes.LNat L.
+Require Import Nat.
 
 (** ** Decidabiity of closedness, boundedness and procness *)
 
